part2: try to solve pop

heap/tree_pop.v
@@ -15,14 +15,15 @@ Require Import cprogs.heap.list_relation.
 Require Import cprogs.heap.definitions.
 Require Import cprogs.heap.tree_list.
 Require Import cprogs.heap.tree_down.
+Require Import cprogs.heap.tree_push.
 
 Fixpoint tree_to_partial_tree_pop_fix (tl: partial_tree) (t: tree) (d: Z): partial_tree :=
   match t with
     | Leaf => tl
     | Node v ls rs => 
       match (full_tree_b (d - 2) rs) with
-      | false => tree_to_partial_tree_pop_fix ((false, v, ls) :: tl) rs (d-1)
-      | true => tree_to_partial_tree_pop_fix ((true, v, rs) :: tl) ls (d-1)
+      | false => tree_to_partial_tree_pop_fix ((true, v, ls) :: tl) rs (d-1)
+      | true => tree_to_partial_tree_pop_fix ((false, v, rs) :: tl) ls (d-1)
       end (*true go right and right is cut*)
   end.
 
@@ -32,7 +33,7 @@ Definition tree_to_partial_tree_pop(t: tree) (d: Z): partial_tree :=
 Definition get_last_val(l: partial_tree): Z :=
   match l with
     | nil => 0
-    | (flg, v, tr)::lt => v
+    | (flg, v, tr) :: lt => v
   end.
 
 Definition tree_cut_last(ls rs: tree) (d: Z): tree :=
@@ -57,10 +58,309 @@ Lemma tree_not_emp: forall (t: tree),
 Proof.
 Admitted.
 
-Lemma MaxHeap_tree_down_state: forall (ls rs: tree) (d v: Z),
-  MaxHeap (Node v ls rs) -> complete_tree_pop d (Node v ls rs) -> MaxHeap_tree_down ([], tree_cut_last ls rs d).
+Lemma MaxHeap_tree_partial_tree_skip: forall (lt: partial_tree),
+  MaxHeap_partial_tree lt -> MaxHeap_partial_tree (skipn 1 lt).
 Proof.
-Admitted.
+  intros.
+  induction lt.
+  + simpl; tauto.
+  + destruct a as [[flg val] tr].
+    inversion H.
+    simpl.
+    apply (MaxHeap_partial_tree_v_impl _ val).
+    tauto.
+Qed.
+
+Lemma tree_to_partial_tree_pop_get: forall (t tr: tree) (lt: partial_tree) (flg: bool) (v d: Z), 
+  tree_to_partial_tree_pop_fix (lt ++ [(flg,v,tr)]) t d = (tree_to_partial_tree_pop_fix lt t d) ++ [(flg,v,tr)].
+Proof.
+  intros.
+  revert v tr flg d lt.
+  induction t; intros.
+  + unfold tree_to_partial_tree_pop_fix; tauto.
+  + simpl.
+    destruct (full_tree_b (d - 2) t2).
+    - replace ((false, v, t2) :: (lt ++ [(flg, v0, tr)])) with ([(false, v, t2)] ++ (lt ++ [(flg, v0, tr)])) by reflexivity.
+      replace ((false, v, t2) :: lt) with ([(false, v, t2)] ++ lt) by reflexivity.
+      rewrite app_assoc.
+      apply IHt1.
+    - replace ((true, v, t1) :: (lt ++ [(flg, v0, tr)])) with ([(true, v, t1)] ++ (lt ++ [(flg, v0, tr)])) by reflexivity.
+      replace ((true, v, t1) :: lt) with ([(true, v, t1)] ++ lt) by reflexivity.
+      rewrite app_assoc.
+      apply IHt2.
+Qed.
+
+Lemma MaxHeap_tree_partial_hold: forall (t: tree) (d: Z) (lt: partial_tree),
+  complete_tree_pop d t -> MaxHeap t -> (t = Leaf \/ MaxHeap_partial_tree_v lt (get_tree_val t)) -> MaxHeap_partial_tree lt -> 
+  MaxHeap_partial_tree (tree_to_partial_tree_pop_fix lt t d).
+Proof.
+  intros.
+  revert lt d H H2 H1.
+  induction H0; intros; subst.
+  + simpl; tauto.
+  + simpl; inversion H2; subst.
+    - apply full_tree_equiv1 in H8.
+      rewrite H8.
+      destruct H4; [discriminate|unfold get_tree_val in H].
+      apply IHMaxHeap1; [tauto| | ].
+      * unfold MaxHeap_partial_tree; tauto.
+      * destruct H0; [left; tauto|right].
+        eapply MaxHeap_partial_tree_v_app; try reflexivity; try tauto.
+    - pose proof complete_tree_pop_not_fullb _ _ H8.
+      replace (d-1-1) with (d-2) in H by lia.
+      rewrite H.
+      destruct H4; [discriminate|unfold get_tree_val in H4].
+      apply IHMaxHeap2; [tauto| | ].
+      * unfold MaxHeap_partial_tree; tauto.
+      * destruct H1; [left; tauto|right].
+        eapply MaxHeap_partial_tree_v_app; try reflexivity; try tauto.
+Qed.
+
+Lemma tree_to_partial_tree_len: forall (t: tree) (d: Z),
+  t <> Leaf -> 1 <= Zlength (tree_to_partial_tree_pop t d).
+Proof.
+  intros.
+  revert d.
+  induction t; [tauto|].
+  intros.
+  unfold tree_to_partial_tree_pop; simpl.
+  destruct (full_tree_b (d-2) t2); simpl.
+  + replace ((false, v, t2) :: nil) with (nil ++ [(false, v, t2)]); [|rewrite app_nil_l; tauto].
+    rewrite tree_to_partial_tree_pop_get.
+    rewrite Zlength_app.
+    replace (Zlength [(false, v, t2)]) with 1 by tauto.
+    pose proof initial_world.zlength_nonneg _ (tree_to_partial_tree_pop_fix [] t1 (d - 1)).
+    lia.
+  + replace ((true, v, t1) :: nil) with (nil ++ [(true, v, t1)]); [|rewrite app_nil_l; tauto].
+    rewrite tree_to_partial_tree_pop_get.
+    rewrite Zlength_app.
+    replace (Zlength [(true, v, t1)]) with 1 by tauto.
+    pose proof initial_world.zlength_nonneg _ (tree_to_partial_tree_pop_fix [] t2 (d - 1)).
+    lia.
+Qed.
+
+Lemma full_tree_gt_0: forall (t: tree) (d: Z),
+  full_tree d t -> d >= 0.
+Proof.
+  intros.
+  induction H.
+  + lia.
+  + lia.
+Qed.
+
+Lemma tree_compose_size_pop: forall (t: tree) (d: Z),
+  complete_tree_pop d t -> t <> Leaf -> tree_size
+  (tree_compose (skipn 1 (tree_to_partial_tree_pop t d)) Leaf) + 1 = tree_size t.
+Proof.
+  intros.
+  revert d H.
+  induction t; intros; [tauto|].
+  unfold tree_to_partial_tree_pop.
+  inversion H; subst.
+  + apply full_tree_equiv1 in H5.
+    unfold tree_to_partial_tree_pop_fix; fold tree_to_partial_tree_pop_fix.
+    rewrite H5.
+    destruct t1.
+    - inversion H3.
+      replace (d-2) with (-1) in H5 by lia.
+      apply full_tree_equiv1 in H5.
+      pose proof full_tree_gt_0 _ _ H5.
+      lia. 
+    - replace ((false, v, t2) :: nil) with (nil ++ [(false, v, t2)]); [|rewrite app_nil_l; tauto].
+      rewrite tree_to_partial_tree_pop_get.
+      replace 1%nat with (Z.to_nat 1) by lia.
+      pose proof tree_to_partial_tree_len (Node v0 t1_1 t1_2) (d-1).
+      unfold tree_to_partial_tree_pop in H1.
+      rewrite Zskipn_app1; [|apply H1; discriminate].
+      rewrite tree_compose_append.
+      unfold tree_size; fold tree_size.
+      unfold tree_to_partial_tree_pop in IHt1.
+      replace (Z.to_nat 1) with 1%nat by lia.
+      specialize (IHt1 ltac:(discriminate) (d-1) H3).
+      replace (tree_size (tree_compose (skipn 1 (tree_to_partial_tree_pop_fix [] (Node v0 t1_1 t1_2) (d - 1))) Leaf)) with (tree_size (Node v0 t1_1 t1_2) - 1) by lia.
+      simpl; lia.
+  + pose proof complete_tree_pop_not_fullb _ _ H5.
+    unfold tree_to_partial_tree_pop_fix; fold tree_to_partial_tree_pop_fix.
+    replace (d-1-1) with (d-2) in H1 by lia.
+    rewrite H1.
+    destruct t2.
+    - simpl.
+      inversion H3; [simpl; tauto|].
+      inversion H5.
+      replace (d-1-1) with (-1) in H2 by lia.
+      pose proof full_tree_gt_0 _ _ H2; lia.
+    - replace ((true, v, t1) :: nil) with (nil ++ [(true, v, t1)]); [|  rewrite app_nil_l; tauto].
+      rewrite tree_to_partial_tree_pop_get.
+      replace 1%nat with (Z.to_nat 1) by lia.
+      pose proof tree_to_partial_tree_len (Node v0 t2_1 t2_2) (d-1).
+      unfold tree_to_partial_tree_pop in H2.
+      rewrite Zskipn_app1; [|apply H2; discriminate].
+      rewrite tree_compose_append.
+      unfold tree_size; fold tree_size.
+      unfold tree_to_partial_tree_pop in IHt2.
+      replace (Z.to_nat 1) with 1%nat by lia.
+      specialize (IHt2 ltac:(discriminate) (d-1) H5).
+      replace (tree_size (tree_compose (skipn 1 (tree_to_partial_tree_pop_fix [] (Node v0 t2_1 t2_2) (d - 1))) Leaf)) with (tree_size (Node v0 t2_1 t2_2) - 1) by lia.
+      simpl; lia.
+Qed.
+
+Lemma tree_cut_last_size: forall (ls rs: tree) (v d: Z),
+  tree_size (Node v ls rs) >= 2 -> complete_tree_pop d (Node v ls rs) -> tree_size (tree_cut_last ls rs d) = tree_size ls + tree_size rs.
+Proof.
+  intros.
+  unfold tree_cut_last.
+  inversion H0; subst. 
+  + apply full_tree_equiv1 in H5; rewrite H5.
+    unfold tree_size; fold tree_size.
+    inversion H3.
+    - replace (d-2) with (-1) in H5 by lia; apply full_tree_equiv1 in H5.
+      pose proof full_tree_gt_0 _ _ H5; lia.
+    - assert (ls <> Leaf); [rewrite <- H4;discriminate|].
+      pose proof tree_compose_size_pop _ _ H3 H6.
+      rewrite <- H4 in H7.
+      replace (tree_size (tree_compose (skipn 1 (tree_to_partial_tree_pop (Node v0 ls0 rs0) (d - 1))) Leaf)) with (tree_size (Node v0 ls0 rs0) - 1) by lia.
+      lia.
+    - assert (ls <> Leaf); [rewrite <- H4;discriminate|].
+      pose proof tree_compose_size_pop _ _ H3 H6.
+      rewrite <- H4 in H7.
+      replace (tree_size (tree_compose (skipn 1 (tree_to_partial_tree_pop (Node v0 ls0 rs0) (d - 1))) Leaf)) with (tree_size (Node v0 ls0 rs0) - 1) by lia.
+      lia.
+  + pose proof complete_tree_pop_not_fullb _ _ H5.
+    replace (d-1-1) with (d-2) in H1 by lia; rewrite H1.
+    unfold tree_size; fold tree_size.
+    inversion H5.
+    - rewrite H2 in H3; inversion H3.
+      assert (tree_size (Node v ls rs) = 1); [simpl;rewrite <- H4; rewrite <- H7; tauto | ].
+      lia.
+      pose proof full_tree_gt_0 _ _ H6; lia.
+    - assert (rs <> Leaf); [rewrite <- H6;discriminate|].
+      pose proof tree_compose_size_pop _ _ H5 H7.
+      rewrite <- H6 in H8.
+      replace (tree_size (tree_compose (skipn 1 (tree_to_partial_tree_pop (Node v0 ls0 rs0) (d - 1))) Leaf)) with (tree_size (Node v0 ls0 rs0) - 1) by lia.
+      lia.
+    - assert (rs <> Leaf); [rewrite <- H6;discriminate|].
+      pose proof tree_compose_size_pop _ _ H5 H7.
+      rewrite <- H6 in H8.
+      replace (tree_size (tree_compose (skipn 1 (tree_to_partial_tree_pop (Node v0 ls0 rs0) (d - 1))) Leaf)) with (tree_size (Node v0 ls0 rs0) - 1) by lia.
+      lia.
+Qed.
+
+Lemma MaxHeap_tree_down_state: forall (ls rs: tree) (d v: Z),
+  tree_size (Node v ls rs) >= 2 -> MaxHeap (Node v ls rs) -> complete_tree_pop d (Node v ls rs) ->
+  MaxHeap_tree_down ([], tree_cut_last ls rs d).
+Proof.
+  intros.
+  unfold MaxHeap_tree_down; simpl.
+  split; [apply MaxHeap_partial_tree_v_nil; reflexivity|].
+  split.
+  + unfold tree_cut_last.
+    inversion H0; [discriminate|].
+    unfold MaxHeap_no_rt.
+    inversion H1; subst.
+    - apply full_tree_equiv1 in H11.
+      rewrite H11.
+      exists (get_last_val (tree_to_partial_tree_pop ls (d - 1))), (tree_compose (skipn 1 (tree_to_partial_tree_pop ls (d - 1))) Leaf), rs.
+      injection H2; intros; subst.
+      split; [tauto|].
+      split; [|tauto].
+      apply tree_compose_MaxHeap; [apply MaxHeap_Leaf; tauto|left].
+      split; [reflexivity|].
+      apply MaxHeap_tree_partial_tree_skip.
+      unfold tree_to_partial_tree_pop.
+      apply MaxHeap_tree_partial_hold; try tauto; [|unfold MaxHeap_partial_tree; tauto].
+      destruct H5; [left;tauto|right].
+      apply MaxHeap_partial_tree_v_nil.
+      reflexivity.
+    - pose proof complete_tree_pop_not_fullb _ _ H11.
+      replace (d-1-1) with (d-2) in H7 by lia.
+      rewrite H7.
+      exists (get_last_val (tree_to_partial_tree_pop rs (d - 1))), ls, (tree_compose (skipn 1 (tree_to_partial_tree_pop rs (d - 1))) Leaf).
+      injection H2; intros; subst.
+      split; [tauto|].
+      split; [tauto|].
+      apply tree_compose_MaxHeap; [apply MaxHeap_Leaf; tauto|left].
+      split; [reflexivity|].
+      apply MaxHeap_tree_partial_tree_skip.
+      unfold tree_to_partial_tree_pop.
+      apply MaxHeap_tree_partial_hold; try tauto; [|unfold MaxHeap_partial_tree; tauto].
+      destruct H6; [left;tauto|right].
+      apply MaxHeap_partial_tree_v_nil.
+      reflexivity.
+  + pose proof tree_cut_last_size ls rs v d H H1.
+    simpl in H.
+    pose proof tree_not_emp (tree_cut_last ls rs d) ltac:(lia).
+    destruct H3 as [v0 [ls0 [rs0]]].
+    exists v0, ls0, rs0.
+    split; [tauto|].
+    split; right; apply MaxHeap_partial_tree_v_nil; tauto.
+Qed.
+
+Lemma complete_tree_pop_holds: forall (t: tree)(d: Z), 
+   t <> Leaf -> complete_tree_pop d t -> complete_tree_push d (tree_compose (skipn 1%nat (tree_to_partial_tree_pop t d)) Leaf).
+Proof.
+  intros.
+  induction H0.
+  + tauto.
+  + unfold tree_to_partial_tree_pop.
+    unfold tree_to_partial_tree_pop_fix; fold tree_to_partial_tree_pop_fix.
+    apply full_tree_equiv1 in H1; rewrite H1.
+    apply full_tree_equiv1 in H1.
+    destruct ls.
+    - inversion H0.
+      replace (dep-2) with (-1) in H1 by lia.
+      pose proof full_tree_gt_0 _ _ H1; lia.
+    - replace ((false, v, rs) :: nil) with (nil ++ [(false, v, rs)]); [|  rewrite app_nil_l; tauto].
+      rewrite tree_to_partial_tree_pop_get.
+      pose proof tree_to_partial_tree_len (Node v0 ls1 ls2) (dep - 1) ltac:(discriminate).
+      replace 1%nat with (Z.to_nat 1) by lia.
+      rewrite Zskipn_app1; [|unfold tree_to_partial_tree_pop in H2; lia].
+      rewrite tree_compose_append.
+      apply complete_tree_push_right_full; [|tauto].
+      apply IHcomplete_tree_pop; discriminate.
+  + unfold tree_to_partial_tree_pop.
+    unfold tree_to_partial_tree_pop_fix; fold tree_to_partial_tree_pop_fix.
+    pose proof complete_tree_pop_not_fullb _ _ H1.
+    replace (dep-1-1) with (dep-2) in H2 by lia; rewrite H2.
+    destruct rs.
+    - inversion H1.
+      simpl.
+      replace dep with 1 by lia.
+      apply complete_tree_push_Leaf; lia.
+    - replace ((true, v, ls) :: nil) with (nil ++ [(true, v, ls)]); [|  rewrite app_nil_l; tauto].
+      rewrite tree_to_partial_tree_pop_get.
+      pose proof tree_to_partial_tree_len (Node v0 rs1 rs2) (dep - 1) ltac:(discriminate).
+      replace 1%nat with (Z.to_nat 1) by lia.
+      rewrite Zskipn_app1; [|unfold tree_to_partial_tree_pop in H3; lia].
+      rewrite tree_compose_append.
+      apply complete_tree_push_left_full; [tauto|].
+      apply IHcomplete_tree_pop; discriminate.
+Qed. 
+
+Lemma complete_tree_pop_holds_all: forall (ls rs: tree)(d v: Z), 
+   complete_tree_pop d (Node v ls rs) -> tree_size (Node v ls rs) >= 2 -> complete_tree_push d (tree_cut_last ls rs d).
+Proof.
+  intros.
+  rename H0 into HH.
+  unfold tree_cut_last.
+  inversion H; subst.
+  + apply full_tree_equiv1 in H4; rewrite H4.
+    apply full_tree_equiv1 in H4.
+    apply complete_tree_push_right_full; [|tauto].
+    apply complete_tree_pop_holds; [|tauto].
+    destruct ls; [|discriminate].
+    inversion H2; replace (d-2) with (-1) in H4 by lia.
+    pose proof full_tree_gt_0 _ _ H4; lia.
+  + pose proof complete_tree_pop_not_fullb _ _ H4.
+    replace (d-1-1) with (d-2) in H0 by lia; rewrite H0.
+    apply complete_tree_push_left_full; [tauto|].
+    apply complete_tree_pop_holds; [|tauto].
+    destruct rs; [|discriminate].
+    inversion H4.
+    rewrite H1 in H2.
+    inversion H2.
+    - rewrite <- H5 in HH; simpl in HH; lia.
+    - pose proof full_tree_gt_0 _ _ H5; lia.
+Qed.
 
 Lemma Pop_tree_list_rel: forall (l l': list Z) (t: tree),
   list_on_tree l t -> heap_pop l l' -> MaxHeap t ->
@@ -94,11 +394,20 @@ Proof.
     destruct H4.
     assert (Zlength (fst (firstn (Z.to_nat (Zlength l - 1))
           (upd_Znth 1 l (Znth (Zlength l - 1) l)), 1)) >= 2). {
-      give_up.
+      simpl.
+      rewrite Zlength_firstn.
+      replace (Z.max 0 (Zlength l -1)) with (Zlength l -1) by lia.
+      rewrite upd_Znth_Zlength; [|lia].
+      lia.
     }
     pose proof Down_tree_list_rel _ _ _ H6 H4 H2.
     subst.
-    pose proof MaxHeap_tree_down_state _ _ _ _ H1 H5.
+    assert (tree_size (Node v ls rs) >= 2). {
+      destruct H, H3.
+      rewrite H3; lia.
+    }
+    rename H3 into HH.
+    pose proof MaxHeap_tree_down_state _ _ _ _ HH H1 H5.
     specialize (H7 H3).
     destruct H7 as [t'].
     destruct H7, H8.
@@ -110,4 +419,4 @@ Proof.
     unfold tree_pop; right.
     exists v, ls, rs, t', d.
     tauto.
-Admitted.
+Qed.
